format-version: 1.2
ontology: eo

[Term]
id: EO:0001022
name: gamma radiation treatment
namespace: plant_environment_ontology
def: "A radiation quality treatment (EO:0007154) involving the exposure to gamma radiation." [PO:cooperl]
synonym: "gamma rays" EXACT []
xref: EO_GIT:41
xref: OBO_SF2_EO:41
is_a: EO:0007154  ! radiation quality treatment

[Term]
id: EO:0001039
name: radiation mutagen treatment
namespace: plant_environment_ontology
def: "A radiation treatment (EO:0007151) involving exposure of plant to chemicals or radiation resulting in perturbations to the genome." [PO:cooperl]
xref: EO_GIT:42
xref: OBO_SF2_EO:42
is_a: EO:0007151  ! radiation treatment

[Term]
id: EO:0001040
name: light-induced photooxidative stress treatment
namespace: plant_environment_ontology
def: "A light intensity regimen (EO:0007224) involving use of light-dependent generations of reactive oxygen species." [PO:cooperl]
xref: EO_GIT:44
xref: OBO_SF2_EO:44
is_a: EO:0007224  ! light intensity regimen

[Term]
id: EO:0007001
name: UV-B light regimen
namespace: plant_environment_ontology
def: "The treatment using UV-B light either exclusively or as part of a supplemental electromagnetic radiation in the wavelength range of 315-280nm." [GR:pj]
is_a: EO:0007222  ! UV light regimen

[Term]
id: EO:0007002
name: UV-A light regimen
namespace: plant_environment_ontology
def: "The treatment using UV-A light either exclusively or as part of a supplemental electromagnetic radiation in the wavelength range of 380-315nm." [GR:pj]
is_a: EO:0007222  ! UV light regimen

[Term]
id: EO:0007075
name: high light intensity regimen
namespace: plant_environment_ontology
is_a: EO:0007224  ! light intensity regimen

[Term]
id: EO:0007076
name: moderate light intensity regimen
namespace: plant_environment_ontology
is_a: EO:0007224  ! light intensity regimen

[Term]
id: EO:0007078
name: light quantity regimen
namespace: plant_environment_ontology
def: "In biological experiments often it refer to the length of the exposure time. The treatment also includes the quantity of light falling on a per unit area. This may be expressed either in terms of hours for which teh radiation was available or in the units of luminous flux or the lumens." [GR:pj]
synonym: "photoperiod regimen" RELATED []
is_a: EO:0007153  ! radiation quantity regimen

[Term]
id: EO:0007128
name: intermittent light regimen
namespace: plant_environment_ontology
def: "In biological experiments it refer to the intermittent exposure of plant to the cycles of light and dark or one light Vs the another type of light." [GR:pj]
is_a: EO:0007078  ! light quantity regimen

[Term]
id: EO:0007129
name: UV-C light regimen
namespace: plant_environment_ontology
def: "The treatment using UV-C light either exclusively or as part of a supplemental electromagnetic radiation in the wavelength range of 280-10nm." [GR:pj]
is_a: EO:0007222  ! UV light regimen

[Term]
id: EO:0007130
name: near infra-red light regimen
namespace: plant_environment_ontology
def: "The treatment using infra-red light either exclusively or as part of a supplemental light of near IR band that contains energy in the range of wavelengths 750-1300nm, which is closest to the visible light." [GR:pj]
synonym: "near IR light regimen" RELATED []
is_a: EO:0007202  ! IR light regimen

[Term]
id: EO:0007131
name: middle infra-red light regimen
namespace: plant_environment_ontology
def: "The treatment using middle infra-red light either exclusively or as part of a supplemental light treatment involving middle IR band that contains energy in the range of wavelengths 1300-3000nm." [GR:pj]
is_a: EO:0007202  ! IR light regimen

[Term]
id: EO:0007132
name: far infra-red light regimen
namespace: plant_environment_ontology
def: "The treatment using far infra-red light either exclusively or as part of a supplemental light treatment involving far IR band that contains energy in the range of wavelengths 3000-14000nm." [GR:pj]
is_a: EO:0007202  ! IR light regimen

[Term]
id: EO:0007151
name: radiation treatment
namespace: plant_environment_ontology
def: "A physical plant treatment (EO:0007316) involving an exposure with a radiation type, intensity or quantity." [GR:pj, PO:cooperl]
comment: EMR is classified according to the frequency of its wave. The electromagnetic spectrum, in order of increasing frequency and decreasing wavelength, consists of radio waves, microwaves, infrared radiation, visible light, ultraviolet radiation, X-rays and gamma rays. (from Wikipedia).
synonym: "light regimen" RELATED []
is_a: EO:0007316  ! physical plant treatment

[Term]
id: EO:0007152
name: radiation intensity regimen
namespace: plant_environment_ontology
def: "The treatment involving amount of energy of any radiation incident upon (or flowing through) unit area, perpendicular to the radiation source, in unit time." [GR:pj]
is_a: EO:0007151  ! radiation treatment

[Term]
id: EO:0007153
name: radiation quantity regimen
namespace: plant_environment_ontology
def: "In biological experiments it refer to the treatment involving radiation in terms of length of the exposure time. It also includes the quantity of radiation falling on a per unit area. This is expressed in the units of luminous flux or the lumens." [GR:pj]
is_a: EO:0007151  ! radiation treatment

[Term]
id: EO:0007154
name: radiation quality treatment
namespace: plant_environment_ontology
def: "The treatment involving an exposure to a given type of radiation. Often it is in the form of electromagnetic and ionizing radiation such as light (infrared, visible or ultraviolet), x-rays, gamma rays, etc." [GR:pj]
is_a: EO:0007151  ! radiation treatment

[Term]
id: EO:0007162
name: continuous light regimen
namespace: plant_environment_ontology
def: "The treatment involving continuous exposure of light to the plant." [GR:pj]
is_a: EO:0007078  ! light quantity regimen

[Term]
id: EO:0007163
name: day light regimen
namespace: plant_environment_ontology
def: "The treatment involving an exposure of plant to the scheduled or natural exposure of day light and night cycles to the plant." [GR:pj]
is_a: EO:0007128  ! intermittent light regimen

[Term]
id: EO:0007193
name: day light intensity
namespace: plant_environment_ontology
is_a: EO:0007224  ! light intensity regimen

[Term]
id: EO:0007196
name: light regimen
namespace: plant_environment_ontology
alt_id: EO:0007201
def: "The treatment involving day light as the light of the sun or the artificial light in a growth chamber." [GR:pj]
comment: A type of light used in a commercial light box to simulate natural daylight. For experiments carried out in growth chambers, the daylight is a light source providing a color temperature of 6500+/-200 K at an illumination of 90 to 120 ft/candles. This source is typically provided by fluorescent,  tungsten or halogen lamps.
synonym: "artificial daylight" RELATED []
synonym: "artificial light" RELATED []
synonym: "day light" RELATED []
synonym: "natural light" RELATED []
synonym: "sun light" RELATED []
is_a: EO:0007154  ! radiation quality treatment

[Term]
id: EO:0007199
name: long day length regimen
namespace: plant_environment_ontology
def: "The treatment involving exposure of plant to long day light duration followed by a short night cycle." [GR:pj]
is_a: EO:0007128  ! intermittent light regimen

[Term]
id: EO:0007200
name: short day length regimen
namespace: plant_environment_ontology
def: "The treatment involving exposure of plant to short day light duration followed by a long night cycle." [GR:pj]
is_a: EO:0007128  ! intermittent light regimen

[Term]
id: EO:0007202
name: IR light regimen
namespace: plant_environment_ontology
def: "The treatment using infra red (IR) light either exclusively or as part of a supplemental light treatment involving IR light in the wavelength range of 700nm-1mm." [GR:pj]
is_a: EO:0007196  ! light regimen

[Term]
id: EO:0007203
name: far red light regimen
namespace: plant_environment_ontology
def: "The treatment using far red light either exclusively or as part of a supplemental light treatment involving red color light in the wavelength range of 800-700 nM." [GR:pj]
synonym: "Pfr light" RELATED []
is_a: EO:0007196  ! light regimen

[Term]
id: EO:0007207
name: red light regimen
namespace: plant_environment_ontology
def: "The treatment using red light either exclusively or as part of a supplemental light treatment involving red color light in the wavelength range of 780-622 nM." [GR:pj]
synonym: "Pr light" RELATED []
is_a: EO:0007221  ! visible light regimen

[Term]
id: EO:0007215
name: orange light regimen
namespace: plant_environment_ontology
def: "The treatment using orange light either exclusively or as part of a supplemental light treatment involving orange color light in the wavelength range of 622-597 nM." [GR:pj]
is_a: EO:0007221  ! visible light regimen

[Term]
id: EO:0007216
name: yellow light regimen
namespace: plant_environment_ontology
def: "The treatment using yellow light either exclusively or as part of a supplemental light treatment involving yellow color light in the wavelength range of 597-577 nM." [GR:pj]
is_a: EO:0007221  ! visible light regimen

[Term]
id: EO:0007217
name: green light regimen
namespace: plant_environment_ontology
def: "The treatment using green light either exclusively or as part of a supplemental light treatment involving green color light in the wavelength range of 577-492 nM." [GR:pj]
is_a: EO:0007221  ! visible light regimen

[Term]
id: EO:0007218
name: blue light regimen
namespace: plant_environment_ontology
def: "The treatment using blue light either exclusively or as part of a supplemental light treatment involving blue color light in the wavelength range of 492-455 nM." [GR:pj]
is_a: EO:0007221  ! visible light regimen

[Term]
id: EO:0007219
name: indigo light regimen
namespace: plant_environment_ontology
def: "The treatment using indigo light either exclusively or as part of a supplemental light treatment involving indigo color light in the wavelength range of 450-440 nM." [GR:pj]
is_a: EO:0007221  ! visible light regimen

[Term]
id: EO:0007220
name: violet light regimen
namespace: plant_environment_ontology
def: "The treatment using violet light either exclusively or as part of a supplemental light treatment involving violet color light in the wavelength range of 455-390 nM." [GR:pj]
is_a: EO:0007221  ! visible light regimen

[Term]
id: EO:0007221
name: visible light regimen
namespace: plant_environment_ontology
def: "The treatment using visible light in the wavelength range of 380-780 nM." [GR:pj]
comment: Visible light  is the portion of the electromagnetic spectrum that is visible to the human eye. The optical spectrum is a composite, or mixture, of the various colors.
is_a: EO:0007196  ! light regimen

[Term]
id: EO:0007222
name: UV light regimen
namespace: plant_environment_ontology
def: "The treatment using UV-B light either exclusively or as part of a supplemental light involving electromagnetic radiation in the wavelength range of 315-10nm." [GR:pj]
is_a: EO:0007196  ! light regimen

[Term]
id: EO:0007224
name: light intensity regimen
namespace: plant_environment_ontology
def: "The treatment involving exposure of plant or a plant part to the amount of light energy incident upon (or flowing through) unit area, perpendicular to the radiation source, in unit time." [GR:pj]
is_a: EO:0007152  ! radiation intensity regimen

[Term]
id: EO:0007270
name: continuous dark (no light) regimen
namespace: plant_environment_ontology
def: "The treatment involving continuous exposure to darkness (no light) to the plant." [GR:pj]
synonym: "continuous night regimen" RELATED []
is_a: EO:0007078  ! light quantity regimen

[Term]
id: EO:0007271
name: low light intensity regimen
namespace: plant_environment_ontology
is_a: EO:0007224  ! light intensity regimen

[Term]
id: EO:0007610
name: 3-H
namespace: plant_environment_ontology
synonym: "tritium" RELATED []
is_a: EO:0007154  ! radiation quality treatment

[Term]
id: EO:0007611
name: 3-H-deoxycytidine
namespace: plant_environment_ontology
is_a: EO:0007154  ! radiation quality treatment

[Term]
id: EO:0007612
name: 3-H-thymidine
namespace: plant_environment_ontology
is_a: EO:0007154  ! radiation quality treatment

[Term]
id: EO:0007613
name: 32-P
namespace: plant_environment_ontology
is_a: EO:0007154  ! radiation quality treatment

[Term]
id: EO:0007614
name: agr ray
namespace: plant_environment_ontology
is_a: EO:0007154  ! radiation quality treatment

[Term]
id: EO:0007615
name: Bevatron irradiation
namespace: plant_environment_ontology
is_a: EO:0007154  ! radiation quality treatment

[Term]
id: EO:0007616
name: deuteron irradiation
namespace: plant_environment_ontology
is_a: EO:0007154  ! radiation quality treatment

[Term]
id: EO:0007617
name: ggr ray
namespace: plant_environment_ontology
is_a: EO:0007154  ! radiation quality treatment

[Term]
id: EO:0007618
name: 137-Cs or ggr ray
namespace: plant_environment_ontology
is_a: EO:0007617  ! ggr ray

[Term]
id: EO:0007619
name: 226-Ra or agr ray
namespace: plant_environment_ontology
synonym: "radium" RELATED []
is_a: EO:0007617  ! ggr ray

[Term]
id: EO:0007620
name: 60-Co or ggr ray
namespace: plant_environment_ontology
is_a: EO:0007617  ! ggr ray

[Term]
id: EO:0007621
name: magnetic field
namespace: plant_environment_ontology
is_a: EO:0007154  ! radiation quality treatment

[Term]
id: EO:0007622
name: neutrons
namespace: plant_environment_ontology
is_a: EO:0007154  ! radiation quality treatment

[Term]
id: EO:0007623
name: 252-Cf fission neutrons
namespace: plant_environment_ontology
is_a: EO:0007622  ! neutrons

[Term]
id: EO:0007624
name: radio wave
namespace: plant_environment_ontology
is_a: EO:0007154  ! radiation quality treatment

[Term]
id: EO:0007625
name: stratosphere exposure
namespace: plant_environment_ontology
is_a: EO:0007154  ! radiation quality treatment

[Term]
id: EO:0007626
name: supersonic-treatment
namespace: plant_environment_ontology
is_a: EO:0007154  ! radiation quality treatment

[Term]
id: EO:0007628
name: X-ray
namespace: plant_environment_ontology
def: "The treatment using X-ray either exclusively or as part of a supplemental electromagnetic radiation in the wavelength range of 5pm-10nm." [GR:pj]
is_a: EO:0007154  ! radiation quality treatment

